cfrontend/Clight.v
@@ -675,7 +675,7 @@ Inductive initial_state (p: program): state -> Prop :=
       Genv.init_mem p = Some m0 ->
       Genv.find_symbol ge p.(prog_main) = Some b ->
       Genv.find_funct_ptr ge b = Some f ->
-      type_of_fundef f = Tfunction Tnil type_int32s cc_default ->
+      type_of_fundef f = Tfunction Tnil type_pint32s cc_default ->
       initial_state p (Callstate f nil Kstop m0).
 
 (** A final state is a [Returnstate] with an empty continuation. *)
