cfrontend/SimplLocals.v
@@ -61,8 +61,8 @@ Definition Sdebug_temp (id: ident) (ty: type) :=
 
 Definition Sdebug_var (id: ident) (ty: type) :=
   Sbuiltin None (EF_debug 5%positive id (AST.Tptr :: nil))
-                (Tcons (Tpointer ty noattr) Tnil)
-                (Eaddrof (Evar id ty) (Tpointer ty noattr) :: nil).
+                (Tcons (Tpointer ty pnoattr) Tnil)
+                (Eaddrof (Evar id ty) (Tpointer ty pnoattr) :: nil).
 
 Definition Sset_debug (id: ident) (ty: type) (a: expr) :=
   if Compopts.debug tt
