extraction/extraction.v
@@ -171,7 +171,7 @@ Separate Extraction
    Cexec.do_initial_state Cexec.do_step Cexec.at_final_state
    Ctypes.merge_attributes Ctypes.remove_attributes Ctypes.build_composite_env
    Initializers.transl_init Initializers.constval
-   Csyntax.Eindex Csyntax.Epreincr
+   Csyntax.Epreincr
    Ctyping.typecheck_program
    Ctyping.epostincr Ctyping.epostdecr Ctyping.epreincr Ctyping.epredecr
    Ctypes.make_program
